get rid of unsafeCoerce in Haskell code
required converting [prog] to be parametrized by the eventual
type of the Done value.

nice side-effect: a cleaner, more modular proof in Idempotent.v.

src/hstest.hs
@@ -7,7 +7,6 @@ import Prog
 import Word
 import qualified Data.ByteString
 import qualified Testprog
-import Unsafe.Coerce
 
 disk_fn :: String
 disk_fn = "disk.img"
@@ -38,19 +37,19 @@ write_disk f (W64 a) (W4096 v) = do
   return ()
 write_disk _ _ _ = error "write_disk: unexpected addr or val"
 
-run_dcode :: Handle -> Prog.Coq_prog -> IO (Prelude.Maybe Word.Coq_word)
-run_dcode _ (Done r) = return $ unsafeCoerce r
+run_dcode :: Handle -> Prog.Coq_prog a -> IO a
+run_dcode _ (Done r) = return r
 run_dcode f (Read a rx) = do val <- read_disk f a; run_dcode f $ rx val
 run_dcode f (Write a v rx) = do write_disk f a v; run_dcode f $ rx ()
 
-the_prog :: Log.Coq_xparams -> Prog.Coq_prog
+the_prog :: Log.Coq_xparams -> Prog.Coq_prog Prelude.Integer
 the_prog xp =
   _LOG__init xp $ \_ ->
   _LOG__begin xp $ \_ ->
   _LOG__read xp (W64 5) $ \v ->
   _LOG__write xp (W64 6) v $ \_ ->
   _LOG__commit xp $ \_ ->
-  Prog.Done $ unsafeCoerce Nothing
+  Prog.Done 0
 
 lxp :: Log.Coq_xparams
 lxp = Log.Build_xparams
@@ -69,8 +68,8 @@ main = do
   putStrLn "Running program.."
   f <- openFile disk_fn ReadWriteMode
   -- r <- run_dcode f $ the_prog lxp
-  -- r <- run_dcode f $ Testprog.testcopy lxp $ Prog.Done $ unsafeCoerce Nothing
-  r <- run_dcode f $ Testprog.testalloc lxp bxp $ \x -> Prog.Done $ unsafeCoerce x
+  -- r <- run_dcode f $ Testprog.testcopy lxp $ Prog.Done Nothing
+  r <- run_dcode f $ Testprog.testalloc lxp bxp $ \x -> Prog.Done x
   hClose f
   putStrLn $ "Done: " ++ (show r)
 
