src/Idempotent.v
@@ -9,22 +9,95 @@ Ltac do_inj_pair2 :=
   | [ H: existT _ _ _ = existT _ _ _ |- _ ] => apply inj_pair2 in H; subst
   end.
 
-Theorem corr2_from_corr3: forall p pre, {{ pre }} p >> Done tt
-  -> {{ fun done crash => pre done (fun _ _ => crash) }} p.
+Theorem corr2_from_corr3: forall T (p: prog T) pre, {{ pre }} p >> Done tt
+  -> {{ fun done crash => pre done (fun _ => crash) }} p.
 Proof.
   unfold corr2; intros.
   destruct out.
   - exfalso.
     edestruct H; eauto; repeat deex; try congruence.
   - edestruct H; eauto; repeat deex.
-    inversion H3; subst; do_inj_pair2.
-    left. repeat eexists; eauto.
+    + inversion H3; subst; do_inj_pair2.
+      left. repeat eexists; eauto.
+    + inversion H3; subst; do_inj_pair2.
   - edestruct H; eauto; repeat deex.
-    inversion H3; subst; do_inj_pair2.
-    right. repeat eexists; eauto.
+    + inversion H3; subst; do_inj_pair2.
+    + inversion H3; subst; do_inj_pair2.
+      right. repeat eexists; eauto.
 Qed.
 
-Theorem corr3_from_corr2: forall p r ppre rpre, {{ ppre }} p
+Lemma corr3_from_corr2_failed:
+  forall (TF TR: Set) m (p: prog TF) (r: prog TR) out
+         (crash: pred) ppre rpre crashdone_p crashdone_r,
+  exec_recover m p r out
+  -> TF = TR
+  -> crash m
+  -> (crash ==> ppre crashdone_p crash)
+  -> (crash ==> rpre crashdone_r crash)
+  -> {{ ppre }} p
+  -> {{ rpre }} r
+  -> out <> RFailed TF TR.
+Proof.
+  intros.
+  induction H; try congruence.
+  - edestruct H4; eauto.
+    destruct H6. destruct H6. destruct H6. congruence.
+    destruct H6. destruct H6. congruence.
+  - rewrite H0. eapply IHexec_recover; eauto.
+    edestruct H4; eauto.
+    destruct H7. destruct H7. destruct H7. congruence.
+    destruct H7. destruct H7. inversion H7. congruence.
+Qed.
+
+Lemma corr3_from_corr2_finished:
+  forall (TF TR: Set) m (p: prog TF) (r: prog TR) out
+         (crash: pred) ppre rpre crashdone_p crashdone_r m' v,
+  exec_recover m p r out
+  -> TF = TR
+  -> crash m
+  -> (crash ==> ppre crashdone_p crash)
+  -> (crash ==> rpre crashdone_r crash)
+  -> {{ ppre }} p
+  -> {{ rpre }} r
+  -> out = RFinished TR m' v
+  -> crashdone_p v m'.
+Proof.
+  intros.
+  induction H; try congruence.
+  edestruct H4; eauto.
+  - destruct H7. destruct H7. destruct H7.
+    inversion H7. congruence.
+  - destruct H7. destruct H7. congruence.
+Qed.
+
+Lemma corr3_from_corr2_recovered:
+  forall (TF TR: Set) m (p: prog TF) (r: prog TR) out
+         (crash: pred) ppre rpre crashdone_p crashdone_r m' v,
+  exec_recover m p r out
+  -> TF = TR
+  -> crash m
+  -> (crash ==> ppre crashdone_p crash)
+  -> (crash ==> rpre crashdone_r crash)
+  -> {{ ppre }} p
+  -> {{ rpre }} r
+  -> out = RRecovered TF m' v
+  -> crashdone_r v m'.
+Proof.
+  intros.
+  induction H; try congruence.
+  - eapply corr3_from_corr2_finished; eauto; try congruence.
+    clear IHexec_recover H7.
+    edestruct H4; eauto.
+    + destruct H7. destruct H7. destruct H7. congruence.
+    + destruct H7. destruct H7. congruence.
+  - eapply IHexec_recover; eauto; clear IHexec_recover H7.
+    + edestruct H4; eauto.
+      * destruct H7. destruct H7. destruct H7. congruence.
+      * destruct H7. destruct H7. congruence.
+    + inversion H6. auto.
+Qed.
+
+Theorem corr3_from_corr2: forall TF TR (p: prog TF) (r: prog TR) ppre rpre, {{ ppre }} p
   -> {{ rpre }} r
   -> {{ fun done crashdone => exists crash,
         ppre done crash * [[ crash ==> rpre crashdone crash ]] }} p >> r.
@@ -37,42 +110,20 @@ Proof.
     edestruct H; eauto; repeat deex; try congruence.
   - repeat eexists; intuition eauto; try congruence.
     edestruct H; eauto; repeat deex; try congruence.
-    inversion H7; subst; do_inj_pair2; eauto.
+    inversion H6; subst; do_inj_pair2; eauto.
   - edestruct H; eauto; repeat deex; try congruence.
     inversion H7; clear H7; subst.
     exfalso.
     clear H H1 H2 H4 ppre p done m.
-    assert (exists x, x = r) as Hx by eauto. destruct Hx.
-    rewrite <- H in H5 at 1.
-    assert (exists x, x = RFailed) as Hx by eauto. destruct Hx.
-    rewrite <- H1 in H5.
-    induction H5; subst; try congruence.
-    + edestruct H0; eauto; repeat deex; try congruence.
-    + eapply IHexec_recover; eauto.
-      edestruct H0; eauto; repeat deex; try congruence.
+    eapply corr3_from_corr2_failed; eauto.
   - edestruct H; eauto; repeat deex; try congruence.
     inversion H7; clear H7; subst.
     clear H H1 H2 H4 ppre p m.
-    assert (exists x, x = r) as Hx by eauto. destruct Hx.
-    rewrite <- H in H5 at 1.
-    assert (exists x, x = RFinished c m'' v) as Hx by eauto. destruct Hx.
-    rewrite <- H1 in H5.
-    induction H5; intros; subst; try congruence.
-    + inversion H1; clear H1; subst; do_inj_pair2.
-      repeat eexists; intros; try congruence.
-      edestruct H0; eauto; repeat deex; try congruence.
-      inversion H4; subst; do_inj_pair2.
-      eauto.
-    + inversion H1; clear H1; subst; do_inj_pair2.
-      destruct c0.
-      * clear IHexec_recover.
-        inversion H5; clear H5; subst; do_inj_pair2.
-        edestruct H0; [| eapply H7 | .. ].
-        eapply H3; clear H7.
-        edestruct H0; eauto; repeat deex; try congruence.
-        repeat deex. inversion H1; subst; do_inj_pair2.
-        repeat eexists; intuition eauto; try congruence.
-        repeat deex; try congruence.
-      * eapply IHexec_recover; eauto.
-        edestruct H0; eauto; repeat deex; try congruence.
+    right. exists m''; exists v. intuition.
+    eapply corr3_from_corr2_finished; eauto.
+  - edestruct H; eauto; repeat deex; try congruence.
+    inversion H7; clear H7; subst.
+    clear H H1 H2 H4 ppre p m.
+    right. exists m''; exists v. intuition.
+    eapply corr3_from_corr2_recovered; eauto.
 Qed.
